update the easy cases of Dmajortodflatmajor

src/Dmajortodflatmajor.v
@@ -16,6 +16,8 @@ Require compcert.backend.SelectLong.
 Require oeuf.TraceSemantics.
 Require Import oeuf.FullSemantics.
 Require Import oeuf.OeufMem.
+Require Import oeuf.OpaqueOps.
+Require oeuf.MemInjProps.
 
 Require Import oeuf.Dmajor.
 Require Import oeuf.Dflatmajor.
@@ -84,7 +86,7 @@ Definition env_inj (mi : meminj) (e e' : env) : Prop :=
       e' ! id = Some v' /\ Val.inject mi v v'.
 
 (* globals aren't moved around *)
-Definition globals_inj_same := HighValues.globals_inj_same ge.
+Definition globals_inj_same := MemInjProps.globals_inj_same ge.
 
 (* yet another useful property for a mapping function *)
 Definition meminj_injective (mi : meminj) : Prop :=
@@ -94,7 +96,7 @@ Definition meminj_injective (mi : meminj) : Prop :=
     b1 = b2.
 
 (* nothing is moved around within blocks *)
-Definition same_offsets := HighValues.same_offsets.
+Definition same_offsets := MemInjProps.same_offsets.
 
 (* conglomeration props *)
 Definition wf_inj (mi : meminj) : Prop :=
@@ -290,6 +292,7 @@ Proof.
 Qed.
 
 
+(* Actually returns the successor of the highest block.  Sorry! *)
 Fixpoint highest_block (c : Dflatmajor.cont) : block :=
   match c with
   | Kstop => 1%positive
@@ -298,7 +301,7 @@ Fixpoint highest_block (c : Dflatmajor.cont) : block :=
   | Kcall _ _ sp _ k =>
     let h := highest_block k in
     match sp with
-    | Vptr b _ => Pos.max b h
+    | Vptr b _ => Pos.max (Pos.succ b) h
     | _ => h
     end
   end.
@@ -320,15 +323,15 @@ Inductive match_cont : Dmajor.cont -> Dflatmajor.cont -> meminj -> mem -> Prop :
     match_cont k k' mi m ->
     env_inj mi e e' ->
     stack_frame_wf b (fn_stackspace f) mi m ->
-    Plt (highest_block k') b ->
+    Ple (highest_block k') b ->
     match_cont (Dmajor.Kcall oid f e k) (Dflatmajor.Kcall oid f (Vptr b Int.zero) e' k') mi m.
 
 Inductive match_states : Dmajor.state -> Dflatmajor.state -> Prop :=
 | match_state : forall f s k k' b e e' m m' z mi,
     Mem.inject mi m m' ->
     stack_frame_wf b (fn_stackspace f) mi m' ->
-    Plt (highest_block k') b ->
-    Plt (highest_block k') (Mem.nextblock m') ->
+    Ple (highest_block k') b ->
+    Ple (highest_block k') (Mem.nextblock m') ->
     match_cont k k' mi m' ->
     env_inj mi e e' ->
     wf_mem mi m m' ->
@@ -337,7 +340,7 @@ Inductive match_states : Dmajor.state -> Dflatmajor.state -> Prop :=
       (Dflatmajor.State f s k' (Vptr b Int.zero) e' m' z)
 | match_callstate : forall f args args' k k' m m' z mi,
     Mem.inject mi m m' ->
-    Plt (highest_block k') (Mem.nextblock m') ->
+    Ple (highest_block k') (Mem.nextblock m')->
     match_cont k k' mi m' ->
     wf_mem mi m m' ->
     Val.inject_list mi args args' ->
@@ -346,7 +349,7 @@ Inductive match_states : Dmajor.state -> Dflatmajor.state -> Prop :=
       (Dflatmajor.Callstate f args' k' m' z)
 | match_returnstate : forall v v' k k' m m' z mi,
     Mem.inject mi m m' ->
-    Plt (highest_block k') (Mem.nextblock m') ->
+    Ple (highest_block k') (Mem.nextblock m') ->
     match_cont k k' mi m' ->
     wf_mem mi m m' ->
     Val.inject mi v v' ->
@@ -372,30 +375,30 @@ Proof.
   induction 1; intros; simpl; eauto; try solve [econstructor; eauto].
 Qed.
 
-Lemma Plt_pos_max_r :
+Lemma Ple_pos_max_r :
   forall x y z,
-    Plt (Pos.max x y) z ->
-    Plt y z.
+    Ple (Pos.max x y) z ->
+    Ple y z.
 Proof.
   intros.
   destruct (Pos.max_spec x y);
     break_and;
   rewrite H1 in *; eauto.
-  unfold Plt in *.
-  eapply Pos.le_lt_trans; eauto.
+  unfold Ple in *.
+  eapply Pos.le_trans; eauto.
 Qed.
   
-Lemma Plt_pos_max_l :
+Lemma Ple_pos_max_l :
   forall x y z,
-    Plt (Pos.max x y) z ->
-    Plt x z.
+    Ple (Pos.max x y) z ->
+    Ple x z.
 Proof.
   intros.
   destruct (Pos.max_spec x y);
     break_and;
   rewrite H1 in *; eauto.
-  unfold Plt in *.
-  eapply Pos.le_lt_trans; eauto.
+  unfold Ple in *.
+  eapply Pos.le_trans; eauto.
   eapply Pos.lt_eq_cases; eauto.
 Qed.
 
@@ -416,25 +419,35 @@ Proof.
     solve [eauto with mem].
 Qed.
 
+Lemma Ple_succ_ne : forall n m, Ple (Pos.succ n) m -> n <> m.
+intros.
+eapply Plt_ne.
+eapply Plt_Ple_trans.
+- eapply Plt_succ.
+- eauto.
+Qed.
+
+
+Require Import Psatz.
 
 (* If we free a block higher than the largest stack block, stack is still well formed *)
 Lemma match_cont_free_stack_frame :
   forall k k' m' x b lo hi mi,
     match_cont k k' mi m' ->
     Mem.free m' b lo hi = Some x ->
-    Plt (highest_block k') b ->
+    Ple (highest_block k') b ->
     match_cont k k' mi x.
 Proof.
   induction 1; intros; try solve [ econstructor; eauto].
   simpl in H4.
   assert (b0 <> b).
   {
-    eapply Plt_pos_max_l in H4.
-    eapply Plt_ne in H4; congruence.
+    eapply Ple_pos_max_l in H4.
+    eapply Ple_succ_ne in H4; congruence.
   }
   econstructor; eauto.
   eapply IHmatch_cont; eauto.
-  eapply Plt_pos_max_r; eauto.
+  eapply Ple_pos_max_r; eauto.
   unfold stack_frame_wf in *.
   break_and. split; eauto.
   unfold Mem.range_perm in *. intros.
@@ -465,17 +478,20 @@ Proof.
   split.
   intros. break_match; eauto.
 
-  intro.
-  unfold Mem.range_perm in H.
-  specialize (H 0).
-  unfold Mem.valid_block in *.
-  app Mem.alloc_result Mem.alloc.
-  subst b0.
-  match goal with
-  | [ H : Some _ = Some _ |- _ ] => inv H
-  end.
-  app Plt_ne Plt.
-  eauto with mem.
+  {
+    intro.
+    unfold Mem.range_perm in H.
+    specialize (H 0).
+    unfold Mem.valid_block in *.
+    app Mem.alloc_result Mem.alloc.
+    subst b0.
+    match goal with
+    | [ H : Some _ = Some _ |- _ ] => inv H
+    end.
+    app Plt_ne Plt.
+  }
+
+  { eauto with mem. }
 
   unfold stack_frame_wf in *.
   break_and. split.
@@ -728,7 +744,7 @@ Proof.
 
   (* globals_inj_same *)
   unfold globals_inj_same in *.
-  unfold HighValues.globals_inj_same in *.
+  unfold MemInjProps.globals_inj_same in *.
   intros. eapply H2 in H9.
   break_if; congruence.
 
@@ -748,7 +764,7 @@ Proof.
   eapply H7; eauto.
 
   (* same_offsets *)
-  unfold same_offsets. unfold HighValues.same_offsets.
+  unfold same_offsets. unfold MemInjProps.same_offsets.
   intros.
   break_if; simpl; eauto; congruence.
 
@@ -1010,12 +1026,18 @@ Proof.
     find_rewrite; eauto.
 Qed.
 
-Lemma Plt_highest_block_call_cont :
+Lemma Ple_highest_block_call_cont :
   forall k x,
-    Plt (highest_block k) x ->
-    Plt (highest_block (call_cont k)) x.
+    Ple (highest_block k) x ->
+    Ple (highest_block (call_cont k)) x.
 Proof.
   induction k; intros; simpl; auto.
+Qed.
+
+Lemma Ple_trans_succ : forall n m, Ple n m -> Ple n (Pos.succ m).
+intros.
+eapply Ple_trans; eauto.
+eapply Ple_succ.
 Qed.
 
 
@@ -1070,7 +1092,7 @@ Proof.
     eapply wf_mem_store; eauto.
     rewrite Z.add_0_r in *.
     assumption.
-    
+
   * eexists; split; try eapply plus_one; econstructor; eauto.
     destruct vfp; simpl in *; try congruence.
     unfold Genv.find_funct in *.
@@ -1089,8 +1111,9 @@ Proof.
     simpl.
     unfold stack_frame_wf in *.
     break_and. unfold Mem.valid_block in *.
-    eapply Plt_pos_max; eauto.
+    { rewrite <- Pos.le_succ_l in *. eapply Pos.max_lub; eauto. }
     econstructor; eauto.
+
   * invp external_call.
     invp Val.inject.
     app alloc_store_inject Mem.store.
@@ -1110,7 +1133,7 @@ Proof.
 
     erewrite Mem.nextblock_store; try eapply H13.
     eapply Mem.nextblock_alloc in H12.
-    rewrite H12. eapply Plt_trans_succ; eauto.
+    rewrite H12. eapply Ple_trans_succ; eauto.
     
     eapply match_cont_alloc_store; eauto.
     eapply wf_mem_alloc_not_mapped; eauto.
@@ -1158,6 +1181,8 @@ Proof.
       congruence.
     } 
 
+  * (* opaque op *) admit.
+
   * eexists; split; try eapply plus_one; econstructor; eauto.
     econstructor; eauto.
   * eexists; split; try eapply plus_one; econstructor; eauto.
@@ -1167,22 +1192,25 @@ Proof.
   * app free_stack_frame stack_frame_wf.
     eexists; split; try eapply plus_one; econstructor; eauto.
     erewrite Mem.nextblock_free; eauto.
-    eapply Plt_highest_block_call_cont; eauto.
+    eapply Ple_highest_block_call_cont; eauto.
     eapply match_call_cont; eauto.
     eapply match_cont_free_stack_frame; eauto.
     eapply wf_mem_free_right; eauto.
   * app free_stack_frame stack_frame_wf.
     eexists; split; try eapply plus_one; econstructor; eauto; try eapply match_call_cont; eauto.
     erewrite Mem.nextblock_free; eauto.
-    eapply Plt_highest_block_call_cont; eauto.
+    eapply Ple_highest_block_call_cont; eauto.
     eapply match_cont_free_stack_frame; eauto.
     eapply wf_mem_free_right; eauto.
   * app (alloc_stack_frame (fn_stackspace f)) wf_mem.
-    eexists; split; try eapply plus_one; econstructor; eauto.
+    eexists; split; try eapply plus_one.
+    econstructor; eauto.
 
     app Mem.alloc_result Mem.alloc. subst. eauto.
-    app Mem.nextblock_alloc Mem.alloc. find_rewrite.
-    eapply Plt_trans_succ; eauto.
+    app Mem.nextblock_alloc Mem.alloc.
+
+    econstructor; eauto.
+    { find_rewrite. eapply Ple_trans_succ; eauto. }
     
     eapply match_cont_alloc; eauto.
     
@@ -1192,12 +1220,12 @@ Proof.
     
   * inv H3.
     eexists; split; try eapply plus_one; try econstructor; eauto.
-    simpl in H2. eapply Plt_pos_max_r in H2. eauto.
+    simpl in H2. eapply Ple_pos_max_r in H2. eauto.
     eapply env_inj_set_optvar; eauto.
 
     Unshelve.
     repeat (econstructor; eauto).
-Qed.
+Admitted.
 
 Lemma genv_next_add_globals :
   forall {F V} l (ge : @Genv.t F V),
@@ -1217,21 +1245,6 @@ Proof.
   reflexivity.
   rewrite (Pos.add_comm (Pos.of_nat (S n)) 1) at 2.
   repeat rewrite Pos.add_assoc. reflexivity.
-Qed.
-
-Lemma init_mem_nextblock :
-  forall m,
-    Genv.init_mem prog = Some m ->
-    Plt 1%positive (Mem.nextblock m).
-Proof.
-  intros.
-  app Genv.init_mem_genv_next Genv.init_mem.
-  unfold Genv.globalenv in *.
-  rewrite genv_next_add_globals in H; eauto.
-  simpl in *.  
-  rewrite <- H.
-  break_match; try econstructor; eauto.
-  eapply non_empty.
 Qed.
 
 Lemma alloc_wf_mem :
@@ -1263,7 +1276,7 @@ Lemma wf_mem_refl :
 Proof.
   intros. unfold wf_mem. unfold wf_inj.
   repeat split.
-  unfold globals_inj_same. unfold HighValues.globals_inj_same. intros. unfold Mem.flat_inj.
+  unfold globals_inj_same. unfold MemInjProps.globals_inj_same. intros. unfold Mem.flat_inj.
   destruct H0.
   app Genv.find_funct_ptr_not_fresh Genv.find_funct_ptr.
   unfold Mem.valid_block in *. break_match; try congruence.
@@ -1271,7 +1284,7 @@ Proof.
   unfold Mem.valid_block in *. break_match; try congruence.
   unfold meminj_injective. intros. unfold Mem.flat_inj in *.
   repeat break_match_hyp; try congruence.
-  unfold same_offsets. unfold HighValues.same_offsets. unfold Mem.flat_inj.
+  unfold same_offsets. unfold MemInjProps.same_offsets. unfold Mem.flat_inj.
   intros. break_match_hyp; try congruence.
   unfold total_inj. intros.
   unfold Mem.flat_inj.
@@ -1320,24 +1333,6 @@ Proof.
   auto.
 Qed.
 
-Lemma value_inject_not_empty :
-  forall m hv lv,
-    HighValues.value_inject ge m hv lv ->
-    Plt 1%positive (Mem.nextblock m).
-Proof.
-  intros. inv H;
-  unfold Mem.loadv in *;
-  app Mem.load_valid_access Mem.load;
-  try eapply Mem.valid_access_implies in H0;
-  try eapply Mem.valid_access_valid_block in H0;
-  try solve [econstructor];
-  unfold Mem.valid_block in *;
-  destruct (Mem.nextblock m); simpl;  
-  unfold Plt in *; unfold Pos.lt in *; simpl;
-    unfold Pos.compare in *; simpl in *; try reflexivity;
-      break_match_hyp; try congruence.
-Qed.
-
 Lemma value_inject_val_inject :
   forall m hv lv,
     HighValues.value_inject ge m hv lv ->
@@ -1345,7 +1340,9 @@ Lemma value_inject_val_inject :
 Proof.
   intros.
   unfold Mem.flat_inj.
-  inv H; unfold Mem.loadv in *;
+  inv H; cycle 2.
+    { (* opaque case *) admit. }
+  all: unfold Mem.loadv in *;
     eapply Mem.load_valid_access in H0;
     eapply Mem.valid_access_implies in H0;
     try eapply Mem.valid_access_valid_block in H0;
@@ -1354,7 +1351,7 @@ Proof.
     econstructor; eauto;
       try (break_match; try congruence; try reflexivity);
       rewrite Int.add_zero; reflexivity.
-Qed.
+Admitted.
 
   
 Lemma meminj_value_inject :
@@ -1390,7 +1387,7 @@ Proof.
   split.
   unfold wf_mem.
   split. unfold wf_inj.
-  split. unfold globals_inj_same. unfold HighValues.globals_inj_same. intros.
+  split. unfold globals_inj_same. unfold MemInjProps.globals_inj_same. intros.
   unfold Mem.flat_inj. break_match; try congruence.
 
   destruct H3. unfold Genv.find_funct_ptr in *.
@@ -1402,7 +1399,7 @@ Proof.
   
   split. unfold meminj_injective. intros.
   unfold Mem.flat_inj in *. repeat (break_match_hyp; try congruence).
-  unfold same_offsets. unfold HighValues.same_offsets.
+  unfold same_offsets. unfold MemInjProps.same_offsets.
   intros. unfold Mem.flat_inj in *.
   break_match_hyp; try congruence.
   split. unfold total_inj.
@@ -1439,10 +1436,10 @@ Proof.
   copy H1.
   eapply meminj_value_inject in H1; try eapply H0; eauto.
   break_exists; repeat break_and.
-  split; econstructor; eauto; simpl;
-    try eapply value_inject_not_empty; eauto;
-      try solve [econstructor; eauto].
-Qed.
+  split; econstructor; eauto; simpl.
+  - eapply Pos.le_1_l.
+  - econstructor.
+Qed
 
 Theorem fsim' :
   TraceSemantics.forward_simulation (Dmajor.semantics prog) (Dflatmajor.semantics prog).
