src/Dflatmajor.v
@@ -12,6 +12,7 @@ Require Import compcert.common.Switch.
 Require Import oeuf.TraceSemantics.
 Require Import oeuf.HighValues.
 Require Import oeuf.AllValues.
+Require Import oeuf.OpaqueOps.
 
 Require Import List.
 Import ListNotations.
@@ -223,6 +224,11 @@ Inductive step: state -> trace -> state -> Prop :=
         external_call EF_malloc ge (v :: nil) m t vres m' ->
         step (State f (Salloc id expr) k sp e m z)
            t (State f Sskip k sp (PTree.set id vres e) m' z)
+  | step_opaque_op : forall id op args vargs vret f k sp e m z m',
+      eval_exprlist e m sp args vargs ->
+      opaque_oper_denote_mem_effect op ge m vargs m' vret ->
+      step (State f (SopaqueOp id op args) k sp e m z)
+        E0 (State f Sskip k sp (PTree.set id vret e) m' z)
   | step_seq: forall f s1 s2 k sp e m z,
       step (State f (Sseq s1 s2) k sp e m z)
         E0 (State f s1 (Kseq s2 k) sp e m z)
